use abstraction to prove theorems about length

Low/ScalarMult.v
@@ -62,115 +62,9 @@ Require Import Tweetnacl.Low.M.
 Require Import Tweetnacl.Low.S.
 Require Import Tweetnacl.Low.GetBit.
 Require Import Tweetnacl.Low.Constant.
+Require Export Tweetnacl.Low.ScalarMult_gen.
 
 Open Scope Z.
-
-
-Definition get_a (t:(list Z * list Z * list Z * list Z * list Z * list Z)) : list Z := match t with
-  (a,b,c,d,e,f) => a
-end.
-Definition get_b (t:(list Z * list Z * list Z * list Z * list Z * list Z)) : list Z := match t with
-  (a,b,c,d,e,f) => b
-end.
-Definition get_c (t:(list Z * list Z * list Z * list Z * list Z * list Z)) : list Z := match t with
-  (a,b,c,d,e,f) => c
-end.
-Definition get_d (t:(list Z * list Z * list Z * list Z * list Z * list Z)) : list Z := match t with
-  (a,b,c,d,e,f) => d
-end.
-Definition get_e (t:(list Z * list Z * list Z * list Z * list Z * list Z)) : list Z := match t with
-  (a,b,c,d,e,f) => e
-end.
-Definition get_f (t:(list Z * list Z * list Z * list Z * list Z * list Z)) : list Z := match t with
-  (a,b,c,d,e,f) => f
-end.
-
-Section ScalarRec.
-
-Variable A : list Z -> list Z -> list Z.
-Variable M : list Z -> list Z -> list Z.
-Variable Zub : list Z -> list Z -> list Z.
-Variable Sq : list Z -> list Z.
-Variable _121665: list Z.
-Variable Sel25519 : Z -> list Z -> list Z -> list Z.
-Variable getbit : Z -> list Z -> Z.
-
-Fixpoint montgomery_rec_gen (m : nat) (z a b c d e f x : list Z) : (list Z * list Z * list Z * list Z * list Z * list Z) :=
-  match m with
-  | 0%nat => (a,b,c,d,e,f)
-  | S n => 
-      let r := getbit (Z.of_nat (254 - n)) z in
-      let (a, b) := (Sel25519 r a b, Sel25519 r b a) in
-      let (c, d) := (Sel25519 r c d, Sel25519 r d c) in
-      let e := A a c in
-      let a := Zub a c in
-      let c := A b d in
-      let b := Zub b d in
-      let d := Sq e in
-      let f := Sq a in
-      let a := M c a in
-      let c := M b e in
-      let e := A a c in
-      let a := Zub a c in
-      let b := Sq a in
-      let c := Zub d f in
-      let a := M c _121665 in
-      let a := A a d in
-      let c := M c a in
-      let a := M d f in
-      let d := M b x in
-      let b := Sq e in
-      let r := 0 in
-      let (a, b) := (Sel25519 r a b, Sel25519 r b a) in
-      let (c, d) := (Sel25519 r c d, Sel25519 r d c) in
-      montgomery_rec_gen n z a b c d e f x
-    end.
-
-Definition montgomery_step_gen (m:nat) (z a b c d e f x : list Z) : (list Z * list Z * list Z * list Z * list Z * list Z)  :=
-      let r := getbit (Z.of_nat (254 - m)) z in
-      let (a, b) := (Sel25519 r a b, Sel25519 r b a) in
-      let (c, d) := (Sel25519 r c d, Sel25519 r d c) in
-      let e := A a c in
-      let a := Zub a c in
-      let c := A b d in
-      let b := Zub b d in
-      let d := Sq e in
-      let f := Sq a in
-      let a := M c a in
-      let c := M b e in
-      let e := A a c in
-      let a := Zub a c in
-      let b := Sq a in
-      let c := Zub d f in
-      let a := M c _121665 in
-      let a := A a d in
-      let c := M c a in
-      let a := M d f in
-      let d := M b x in
-      let b := Sq e in
-      let r := 0 in
-      let (a, b) := (Sel25519 r a b, Sel25519 r b a) in
-      let (c, d) := (Sel25519 r c d, Sel25519 r d c) in
-      (a,b,c,d,e,f)
-(*     end. *)
-.
-
-Lemma opt_montgomery_rec_step_gen : forall z a b c d e f x n,
-  montgomery_rec_gen (S n) z a b c d e f x = 
-  montgomery_rec_gen n z 
-  (get_a (montgomery_step_gen n z a b c d e f x))
-  (get_b (montgomery_step_gen n z a b c d e f x))
-  (get_c (montgomery_step_gen n z a b c d e f x))
-  (get_d (montgomery_step_gen n z a b c d e f x))
-  (get_e (montgomery_step_gen n z a b c d e f x))
-  (get_f (montgomery_step_gen n z a b c d e f x))
-  x.
-Proof.
-intros.
-simpl ; reflexivity.
-Qed.
-
-End ScalarRec.
 
 Definition montgomery_step := montgomery_step_gen A M Zub Sq _121665 Sel25519 getbit.
 Definition montgomery_rec := montgomery_rec_gen A M Zub Sq _121665 Sel25519 getbit.
@@ -192,246 +86,222 @@ Qed.
 
 Close Scope Z.
 
-Local Ltac solve_montgomery_step_length :=
-  intros;
-  rewrite /montgomery_step /montgomery_step_gen;
-  rewrite /get_a /get_b /get_c /get_d /get_e /get_f;
+Local Ltac solve_montgomery_step_length := 
+  intros; rewrite /montgomery_step;
   repeat match goal with
-    | _ => orewrite Sel25519_length
-    | _ => orewrite M_length
-    | _ => orewrite Sq_length
-    | _ => orewrite A_length
-    | _ => orewrite Zub_length
-    | _ => orewrite Sel25519_length
-  end ; reflexivity.
+    | _ => apply get_a_montgomery_step_gen_length ; auto
+    | _ => apply get_b_montgomery_step_gen_length ; auto
+    | _ => apply get_c_montgomery_step_gen_length ; auto
+    | _ => apply get_d_montgomery_step_gen_length ; auto
+    | _ => apply get_e_montgomery_step_gen_length ; auto
+    | _ => apply get_f_montgomery_step_gen_length ; auto
+    | _ => apply A_length
+    | _ => apply M_length
+    | _ => apply Zub_length
+    | _ => apply Sq_length
+    | _ => apply Sel25519_length
+  end.
 
 Lemma get_a_montgomery_step_length : forall z a b c d e f x n,
-  length a = 16 ->
-  length b = 16 ->
-  length c = 16 ->
-  length d = 16 ->
-  length e = 16 ->
-  length f = 16 ->
+  length a = 16 -> length b = 16 -> length c = 16 ->
+  length d = 16 -> length e = 16 -> length f = 16 ->
   length x = 16 ->
   length (get_a (montgomery_step n z a b c d e f x)) = 16.
 Proof. solve_montgomery_step_length. Qed.
-
 Lemma get_b_montgomery_step_length : forall z a b c d e f x n,
-  length a = 16 ->
-  length b = 16 ->
-  length c = 16 ->
-  length d = 16 ->
-  length e = 16 ->
-  length f = 16 ->
+  length a = 16 -> length b = 16 -> length c = 16 ->
+  length d = 16 -> length e = 16 -> length f = 16 ->
   length x = 16 ->
   length (get_b (montgomery_step n z a b c d e f x)) = 16.
 Proof. solve_montgomery_step_length. Qed.
-
 Lemma get_c_montgomery_step_length : forall z a b c d e f x n,
-  length a = 16 ->
-  length b = 16 ->
-  length c = 16 ->
-  length d = 16 ->
-  length e = 16 ->
-  length f = 16 ->
+  length a = 16 -> length b = 16 -> length c = 16 ->
+  length d = 16 -> length e = 16 -> length f = 16 ->
   length x = 16 ->
   length (get_c (montgomery_step n z a b c d e f x)) = 16.
 Proof. solve_montgomery_step_length. Qed.
-
 Lemma get_d_montgomery_step_length : forall z a b c d e f x n,
-  length a = 16 ->
-  length b = 16 ->
-  length c = 16 ->
-  length d = 16 ->
-  length e = 16 ->
-  length f = 16 ->
+  length a = 16 -> length b = 16 -> length c = 16 ->
+  length d = 16 -> length e = 16 -> length f = 16 ->
   length x = 16 ->
   length (get_d (montgomery_step n z a b c d e f x)) = 16.
 Proof. solve_montgomery_step_length. Qed.
-
 Lemma get_e_montgomery_step_length : forall z a b c d e f x n,
-  length a = 16 ->
-  length b = 16 ->
-  length c = 16 ->
-  length d = 16 ->
-  length e = 16 ->
-  length f = 16 ->
+  length a = 16 -> length b = 16 -> length c = 16 ->
+  length d = 16 -> length e = 16 -> length f = 16 ->
   length x = 16 ->
   length (get_e (montgomery_step n z a b c d e f x)) = 16.
 Proof. solve_montgomery_step_length. Qed.
-
 Lemma get_f_montgomery_step_length : forall z a b c d e f x n,
-  length a = 16 ->
-  length b = 16 ->
-  length c = 16 ->
-  length d = 16 ->
-  length e = 16 ->
-  length f = 16 ->
+  length a = 16 -> length b = 16 -> length c = 16 ->
+  length d = 16 -> length e = 16 -> length f = 16 ->
   length x = 16 ->
   length (get_f (montgomery_step n z a b c d e f x)) = 16.
 Proof. solve_montgomery_step_length. Qed.
 
 Open Scope Z.
 
-Local Ltac solve_montgomery_step_Zlength :=
-  intros;
-  rewrite /montgomery_step /montgomery_step_gen;
-  rewrite /get_a /get_b /get_c /get_d /get_e /get_f;
+Local Ltac solve_montgomery_step_Zlength := 
+  intros; rewrite /montgomery_step;
   repeat match goal with
-    | _ => orewrite Sel25519_Zlength
-    | _ => orewrite M_Zlength
-    | _ => orewrite Sq_Zlength
-    | _ => orewrite A_Zlength
-    | _ => orewrite Zub_Zlength
-    | _ => orewrite Sel25519_Zlength
-  end ; reflexivity.
+    | _ => apply get_a_montgomery_step_gen_Zlength ; auto
+    | _ => apply get_b_montgomery_step_gen_Zlength ; auto
+    | _ => apply get_c_montgomery_step_gen_Zlength ; auto
+    | _ => apply get_d_montgomery_step_gen_Zlength ; auto
+    | _ => apply get_e_montgomery_step_gen_Zlength ; auto
+    | _ => apply get_f_montgomery_step_gen_Zlength ; auto
+    | _ => apply A_Zlength
+    | _ => apply M_Zlength
+    | _ => apply Zub_Zlength
+    | _ => apply Sq_Zlength
+    | _ => apply Sel25519_Zlength
+  end.
 
 Lemma get_a_montgomery_step_Zlength : forall z a b c d e f x n,
-  Zlength a = 16 ->
-  Zlength b = 16 ->
-  Zlength c = 16 ->
-  Zlength d = 16 ->
-  Zlength e = 16 ->
-  Zlength f = 16 ->
+  Zlength a = 16 -> Zlength b = 16 -> Zlength c = 16 ->
+  Zlength d = 16 -> Zlength e = 16 -> Zlength f = 16 ->
   Zlength x = 16 ->
   Zlength (get_a (montgomery_step n z a b c d e f x)) = 16.
 Proof. solve_montgomery_step_Zlength. Qed.
-
 Lemma get_b_montgomery_step_Zlength : forall z a b c d e f x n,
-  Zlength a = 16 ->
-  Zlength b = 16 ->
-  Zlength c = 16 ->
-  Zlength d = 16 ->
-  Zlength e = 16 ->
-  Zlength f = 16 ->
+  Zlength a = 16 -> Zlength b = 16 -> Zlength c = 16 ->
+  Zlength d = 16 -> Zlength e = 16 -> Zlength f = 16 ->
   Zlength x = 16 ->
   Zlength (get_b (montgomery_step n z a b c d e f x)) = 16.
 Proof. solve_montgomery_step_Zlength. Qed.
-
 Lemma get_c_montgomery_step_Zlength : forall z a b c d e f x n,
-  Zlength a = 16 ->
-  Zlength b = 16 ->
-  Zlength c = 16 ->
-  Zlength d = 16 ->
-  Zlength e = 16 ->
-  Zlength f = 16 ->
+  Zlength a = 16 -> Zlength b = 16 -> Zlength c = 16 ->
+  Zlength d = 16 -> Zlength e = 16 -> Zlength f = 16 ->
   Zlength x = 16 ->
   Zlength (get_c (montgomery_step n z a b c d e f x)) = 16.
 Proof. solve_montgomery_step_Zlength. Qed.
-
 Lemma get_d_montgomery_step_Zlength : forall z a b c d e f x n,
-  Zlength a = 16 ->
-  Zlength b = 16 ->
-  Zlength c = 16 ->
-  Zlength d = 16 ->
-  Zlength e = 16 ->
-  Zlength f = 16 ->
+  Zlength a = 16 -> Zlength b = 16 -> Zlength c = 16 ->
+  Zlength d = 16 -> Zlength e = 16 -> Zlength f = 16 ->
   Zlength x = 16 ->
   Zlength (get_d (montgomery_step n z a b c d e f x)) = 16.
 Proof. solve_montgomery_step_Zlength. Qed.
-
 Lemma get_e_montgomery_step_Zlength : forall z a b c d e f x n,
-  Zlength a = 16 ->
-  Zlength b = 16 ->
-  Zlength c = 16 ->
-  Zlength d = 16 ->
-  Zlength e = 16 ->
-  Zlength f = 16 ->
+  Zlength a = 16 -> Zlength b = 16 -> Zlength c = 16 ->
+  Zlength d = 16 -> Zlength e = 16 -> Zlength f = 16 ->
   Zlength x = 16 ->
   Zlength (get_e (montgomery_step n z a b c d e f x)) = 16.
 Proof. solve_montgomery_step_Zlength. Qed.
-
 Lemma get_f_montgomery_step_Zlength : forall z a b c d e f x n,
-  Zlength a = 16 ->
-  Zlength b = 16 ->
-  Zlength c = 16 ->
-  Zlength d = 16 ->
-  Zlength e = 16 ->
-  Zlength f = 16 ->
+  Zlength a = 16 -> Zlength b = 16 -> Zlength c = 16 ->
+  Zlength d = 16 -> Zlength e = 16 -> Zlength f = 16 ->
   Zlength x = 16 ->
   Zlength (get_f (montgomery_step n z a b c d e f x)) = 16.
 Proof. solve_montgomery_step_Zlength. Qed.
 
 Close Scope Z.
 
-
+Local Ltac solve_montgomery_rec_length := 
+  intros; rewrite /montgomery_rec;
+  repeat match goal with
+    | _ => apply get_a_montgomery_rec_gen_length ; auto
+    | _ => apply get_b_montgomery_rec_gen_length ; auto
+    | _ => apply get_c_montgomery_rec_gen_length ; auto
+    | _ => apply get_d_montgomery_rec_gen_length ; auto
+    | _ => apply get_e_montgomery_rec_gen_length ; auto
+    | _ => apply get_f_montgomery_rec_gen_length ; auto
+    | _ => apply A_length
+    | _ => apply M_length
+    | _ => apply Zub_length
+    | _ => apply Sq_length
+    | _ => apply Sel25519_length
+  end.
 
 Lemma get_a_montgomery_get_length : forall n z a b c d e f x,
-  length a = 16 ->
-  length b = 16 ->
-  length c = 16 ->
-  length d = 16 ->
-  length e = 16 ->
-  length f = 16 ->
+  length a = 16 -> length b = 16 -> length c = 16 ->
+  length d = 16 -> length e = 16 -> length f = 16 ->
   length x = 16 ->
   length (get_a (montgomery_rec n z a b c d e f x)) = 16.
-Proof. induction n; intros ; [assumption|] ; simpl.
-apply IHn ; try assumption ; solve_montgomery_step_length.
-Qed.
-
+Proof. solve_montgomery_rec_length. Qed.
 Lemma get_b_montgomery_get_length : forall n z a b c d e f x,
-  length a = 16 ->
-  length b = 16 ->
-  length c = 16 ->
-  length d = 16 ->
-  length e = 16 ->
-  length f = 16 ->
+  length a = 16 -> length b = 16 -> length c = 16 ->
+  length d = 16 -> length e = 16 -> length f = 16 ->
   length x = 16 ->
   length (get_b (montgomery_rec n z a b c d e f x)) = 16.
-Proof. induction n; intros ; [assumption|] ; simpl.
-apply IHn ; try assumption ; solve_montgomery_step_length.
-Qed.
-
+Proof. solve_montgomery_rec_length. Qed.
 Lemma get_c_montgomery_get_length : forall n z a b c d e f x,
-  length a = 16 ->
-  length b = 16 ->
-  length c = 16 ->
-  length d = 16 ->
-  length e = 16 ->
-  length f = 16 ->
+  length a = 16 -> length b = 16 -> length c = 16 ->
+  length d = 16 -> length e = 16 -> length f = 16 ->
   length x = 16 ->
   length (get_c (montgomery_rec n z a b c d e f x)) = 16.
-Proof. induction n; intros ; [assumption|] ; simpl.
-apply IHn ; try assumption ; solve_montgomery_step_length.
-Qed.
-
+Proof. solve_montgomery_rec_length. Qed.
 Lemma get_d_montgomery_get_length : forall n z a b c d e f x,
-  length a = 16 ->
-  length b = 16 ->
-  length c = 16 ->
-  length d = 16 ->
-  length e = 16 ->
-  length f = 16 ->
+  length a = 16 -> length b = 16 -> length c = 16 ->
+  length d = 16 -> length e = 16 -> length f = 16 ->
   length x = 16 ->
   length (get_d (montgomery_rec n z a b c d e f x)) = 16.
-Proof. induction n; intros ; [assumption|] ; simpl.
-apply IHn ; try assumption ; solve_montgomery_step_length.
-Qed.
-
+Proof. solve_montgomery_rec_length. Qed.
 Lemma get_e_montgomery_get_length : forall n z a b c d e f x,
-  length a = 16 ->
-  length b = 16 ->
-  length c = 16 ->
-  length d = 16 ->
-  length e = 16 ->
-  length f = 16 ->
+  length a = 16 -> length b = 16 -> length c = 16 ->
+  length d = 16 -> length e = 16 -> length f = 16 ->
   length x = 16 ->
   length (get_e (montgomery_rec n z a b c d e f x)) = 16.
-Proof. induction n; intros ; [assumption|] ; simpl.
-apply IHn ; try assumption ; solve_montgomery_step_length.
-Qed.
-
+Proof. solve_montgomery_rec_length. Qed.
 Lemma get_f_montgomery_get_length : forall n z a b c d e f x,
-  length a = 16 ->
-  length b = 16 ->
-  length c = 16 ->
-  length d = 16 ->
-  length e = 16 ->
-  length f = 16 ->
+  length a = 16 -> length b = 16 -> length c = 16 ->
+  length d = 16 -> length e = 16 -> length f = 16 ->
   length x = 16 ->
   length (get_f (montgomery_rec n z a b c d e f x)) = 16.
-Proof. induction n; intros ; [assumption|] ; simpl.
-apply IHn ; try assumption ; solve_montgomery_step_length.
-Qed.
+Proof. solve_montgomery_rec_length. Qed.
 
+Open Scope Z.
 
+Local Ltac solve_montgomery_rec_Zlength := 
+  intros; rewrite /montgomery_rec;
+  repeat match goal with
+    | _ => apply get_a_montgomery_rec_gen_Zlength ; auto
+    | _ => apply get_b_montgomery_rec_gen_Zlength ; auto
+    | _ => apply get_c_montgomery_rec_gen_Zlength ; auto
+    | _ => apply get_d_montgomery_rec_gen_Zlength ; auto
+    | _ => apply get_e_montgomery_rec_gen_Zlength ; auto
+    | _ => apply get_f_montgomery_rec_gen_Zlength ; auto
+    | _ => apply A_Zlength
+    | _ => apply M_Zlength
+    | _ => apply Zub_Zlength
+    | _ => apply Sq_Zlength
+    | _ => apply Sel25519_Zlength
+  end.
+
+Lemma get_a_montgomery_get_Zlength : forall n z a b c d e f x,
+  Zlength a = 16 -> Zlength b = 16 -> Zlength c = 16 ->
+  Zlength d = 16 -> Zlength e = 16 -> Zlength f = 16 ->
+  Zlength x = 16 ->
+  Zlength (get_a (montgomery_rec n z a b c d e f x)) = 16.
+Proof. solve_montgomery_rec_Zlength. Qed.
+Lemma get_b_montgomery_get_Zlength : forall n z a b c d e f x,
+  Zlength a = 16 -> Zlength b = 16 -> Zlength c = 16 ->
+  Zlength d = 16 -> Zlength e = 16 -> Zlength f = 16 ->
+  Zlength x = 16 ->
+  Zlength (get_b (montgomery_rec n z a b c d e f x)) = 16.
+Proof. solve_montgomery_rec_Zlength. Qed.
+Lemma get_c_montgomery_get_Zlength : forall n z a b c d e f x,
+  Zlength a = 16 -> Zlength b = 16 -> Zlength c = 16 ->
+  Zlength d = 16 -> Zlength e = 16 -> Zlength f = 16 ->
+  Zlength x = 16 ->
+  Zlength (get_c (montgomery_rec n z a b c d e f x)) = 16.
+Proof. solve_montgomery_rec_Zlength. Qed.
+Lemma get_d_montgomery_get_Zlength : forall n z a b c d e f x,
+  Zlength a = 16 -> Zlength b = 16 -> Zlength c = 16 ->
+  Zlength d = 16 -> Zlength e = 16 -> Zlength f = 16 ->
+  Zlength x = 16 ->
+  Zlength (get_d (montgomery_rec n z a b c d e f x)) = 16.
+Proof. solve_montgomery_rec_Zlength. Qed.
+Lemma get_e_montgomery_get_Zlength : forall n z a b c d e f x,
+  Zlength a = 16 -> Zlength b = 16 -> Zlength c = 16 ->
+  Zlength d = 16 -> Zlength e = 16 -> Zlength f = 16 ->
+  Zlength x = 16 ->
+  Zlength (get_e (montgomery_rec n z a b c d e f x)) = 16.
+Proof. solve_montgomery_rec_Zlength. Qed.
+Lemma get_f_montgomery_get_Zlength : forall n z a b c d e f x,
+  Zlength a = 16 -> Zlength b = 16 -> Zlength c = 16 ->
+  Zlength d = 16 -> Zlength e = 16 -> Zlength f = 16 ->
+  Zlength x = 16 ->
+  Zlength (get_f (montgomery_rec n z a b c d e f x)) = 16.
+Proof. solve_montgomery_rec_Zlength. Qed.
+
+Close Scope Z.
